books/centaur/fgl/interp-st.lisp
@@ -37,21 +37,14 @@
 (include-book "contexts")
 (include-book "stack")
 (include-book "centaur/fty/bitstruct" :dir :system)
-
-
-(fty::defalist nat-nat-alist :key-type natp :val-type natp :true-listp t)
-
-(defstobj interp-profiler
-  (prof-enabledp :type (satisfies booleanp))
-  (prof-indextable)
-  (prof-totalcount :type (integer 0 *) :initially 0)
-  (prof-nextindex :type (integer 0 *) :initially 0)
-  (prof-array :type (array (unsigned-byte 32) (0)) :initially 0 :resizable t)
-  (prof-stack :type (satisfies nat-nat-alist-p)))
+(include-book "prof")
 
 (fty::defbitstruct interp-flags
   ((intro-bvars booleanp)
-   (intro-synvars booleanp)))
+   (intro-synvars booleanp)
+   (simplify-logic booleanp)))
+
+(acl2::defstobj-clone constraint-pathcond pathcond :prefix "CONSTRAINT-")
 
 (make-event
  `(defconst *interp-st-fields*
@@ -62,7 +55,7 @@
       (constraint :type pathcond)
       (constraint-db :type (satisfies constraint-db-p))
       (prof :type interp-profiler)
-      (backchain-limit :type integer)
+      (backchain-limit :type integer :initially -1)
       (bvar-mode :type t)
       (equiv-contexts :type (satisfies equiv-contextsp))
       (reclimit :type (integer 0 *) :initially 0)
@@ -204,3 +197,391 @@
   :hints(("Goal" :in-theory (enable interp-st->flags))))
 
 (in-theory (disable interp-stp))
+
+
+
+
+
+
+(define interp-st-prof-push (name interp-st)       
+  :returns (new-interp-st)
+  :enabled t
+  (stobj-let
+   ((interp-profiler (interp-st->prof interp-st)))
+   (interp-profiler)
+   (prof-push name interp-profiler)
+   interp-st))
+
+(define interp-st-prof-pop-increment (successp interp-st)
+  :returns (new-interp-st)
+  :enabled t
+  (stobj-let
+   ((interp-profiler (interp-st->prof interp-st)))
+   (interp-profiler)
+   (prof-pop-increment successp interp-profiler)
+   interp-st))
+
+(define interp-st-prof-simple-increment-def (name interp-st)
+  :returns (new-interp-st)
+  :enabled t
+  (stobj-let
+   ((interp-profiler (interp-st->prof interp-st)))
+   (interp-profiler)
+   (prof-simple-increment-def name interp-profiler)
+   interp-st))
+
+(define interp-st-prof-simple-increment-exec (name interp-st)
+  :returns (new-interp-st)
+  :enabled t
+  (stobj-let
+   ((interp-profiler (interp-st->prof interp-st)))
+   (interp-profiler)
+   (prof-simple-increment-exec name interp-profiler)
+   interp-st))
+
+(define interp-st-prof-simple-increment-g (name interp-st)
+  :returns (new-interp-st)
+  :enabled t
+  (stobj-let
+   ((interp-profiler (interp-st->prof interp-st)))
+   (interp-profiler)
+   (prof-simple-increment-g name interp-profiler)
+   interp-st))
+
+(define interp-st-prof-unwind-stack (interp-st)
+  :returns (new-interp-st)
+  :enabled t
+  (stobj-let
+   ((interp-profiler (interp-st->prof interp-st)))
+   (interp-profiler)
+   (prof-unwind-stack interp-profiler)
+   interp-st))
+
+(define interp-st-prof-print-report (interp-st)
+  :enabled t
+  (stobj-let
+   ((interp-profiler (interp-st->prof interp-st)))
+   (res)
+   (prof-print-report interp-profiler)
+   res))
+
+(define interp-st-prof-report (interp-st)
+  :enabled t
+  (stobj-let
+   ((interp-profiler (interp-st->prof interp-st)))
+   (interp-profiler)
+   (prof-report interp-profiler)
+   interp-st))
+
+(define interp-st-prof-reset (interp-st)
+  :returns (new-interp-st)
+  :enabled t
+  (stobj-let
+   ((interp-profiler (interp-st->prof interp-st)))
+   (interp-profiler)
+   (prof-reset interp-profiler)
+   interp-st))
+
+(define interp-st-prof-enable (interp-st)
+  :returns (new-interp-st)
+  :enabled t
+  (stobj-let
+   ((interp-profiler (interp-st->prof interp-st)))
+   (interp-profiler)
+   (update-prof-enabledp t interp-profiler)
+   interp-st))
+
+(define interp-st-prof-disable (interp-st)
+  :returns (new-interp-st)
+  :enabled t
+  (stobj-let
+   ((interp-profiler (interp-st->prof interp-st)))
+   (interp-profiler)
+   (update-prof-enabledp nil interp-profiler)
+   interp-st))
+
+(define interp-st-prof-enabledp (interp-st)
+  :returns (new-interp-st)
+  :enabled t
+  (stobj-let
+   ((interp-profiler (interp-st->prof interp-st)))
+   (enabledp)
+   (prof-enabledp interp-profiler)
+   enabledp))
+
+(define update-interp-st-prof-enabledp ((val booleanp) interp-st)
+  :returns (new-interp-st)
+  :enabled t
+  (stobj-let
+   ((interp-profiler (interp-st->prof interp-st)))
+   (interp-profiler)
+   (update-prof-enabledp val interp-profiler)
+   interp-st))
+
+
+
+
+(define interp-st-bindings (interp-st)
+  :enabled t
+  :inline t
+  (stobj-let ((stack (interp-st->stack interp-st)))
+             (bindings)
+             (stack-bindings stack)
+             bindings))
+
+(define interp-st-minor-bindings (interp-st)
+  :enabled t
+  :inline t
+  (stobj-let ((stack (interp-st->stack interp-st)))
+             (bindings)
+             (stack-minor-bindings stack)
+             bindings))
+
+(define interp-st-stack-frames (interp-st)
+  :enabled t
+  :inline t
+  (stobj-let ((stack (interp-st->stack interp-st)))
+             (frames)
+             (stack-frames stack)
+             frames))
+
+(define interp-st-stack-minor-frames (interp-st)
+  :enabled t
+  :inline t
+  (stobj-let ((stack (interp-st->stack interp-st)))
+             (frames)
+             (stack-minor-frames stack)
+             frames))
+
+(define interp-st-pop-frame (interp-st)
+  :enabled t
+  :inline t
+  :guard (and (< 1 (interp-st-stack-frames interp-st))
+              (eql 1 (interp-st-stack-minor-frames interp-st)))
+  (stobj-let ((stack (interp-st->stack interp-st)))
+             (stack)
+             (stack-pop-frame stack)
+             interp-st))
+
+(define interp-st-pop-minor-frame (interp-st)
+  :enabled t
+  :inline t
+  :guard (< 1 (interp-st-stack-minor-frames interp-st))
+  (stobj-let ((stack (interp-st->stack interp-st)))
+             (stack)
+             (stack-pop-minor-frame stack)
+             interp-st))
+
+(define interp-st-push-scratch ((x gl-object-p)
+                                interp-st)
+  :enabled t
+  :inline t
+  (stobj-let ((stack (interp-st->stack interp-st)))
+             (stack)
+             (stack-push-scratch x stack)
+             interp-st))
+
+(define interp-st-scratch-len (interp-st)
+  :enabled t
+  :inline t
+  (stobj-let ((stack (interp-st->stack interp-st)))
+             (len)
+             (stack-scratch-len stack)
+             len))
+
+(define interp-st-pop-scratch ((n natp)
+                                interp-st)
+  :enabled t
+  :inline t
+  :guard (<= n (interp-st-scratch-len interp-st))
+  (stobj-let ((stack (interp-st->stack interp-st)))
+             (stack)
+             (stack-pop-scratch n stack)
+             interp-st))
+
+(define interp-st-peek-scratch ((n natp)
+                                interp-st)
+  :enabled t
+  :inline t
+  :guard (<= n (interp-st-scratch-len interp-st))
+  (stobj-let ((stack (interp-st->stack interp-st)))
+             (args)
+             (stack-peek-scratch n stack)
+             args))
+
+(define interp-st-add-binding ((var pseudo-var-p)
+                               (val gl-object-p)
+                               interp-st)
+  :enabled t
+  :inline t
+  (stobj-let ((stack (interp-st->stack interp-st)))
+             (stack)
+             (stack-add-binding var val stack)
+             interp-st))
+
+(define interp-st-set-bindings ((bindings gl-object-alist-p)
+                                interp-st)
+  :enabled t
+  :inline t
+  (stobj-let ((stack (interp-st->stack interp-st)))
+             (stack)
+             (stack-set-bindings bindings stack)
+             interp-st))
+
+(define interp-st-add-minor-bindings ((bindings gl-object-alist-p)
+                                      interp-st)
+  :enabled t
+  :inline t
+  (stobj-let ((stack (interp-st->stack interp-st)))
+             (stack)
+             (stack-add-minor-bindings bindings stack)
+             interp-st))
+
+(define interp-st-set-minor-bindings ((bindings gl-object-alist-p)
+                                      interp-st)
+  :enabled t
+  :inline t
+  (stobj-let ((stack (interp-st->stack interp-st)))
+             (stack)
+             (stack-set-minor-bindings bindings stack)
+             interp-st))
+
+(define interp-st-push-frame ((bindings gl-object-alist-p)
+                              interp-st)
+  :enabled t
+  :inline t
+  (stobj-let ((stack (interp-st->stack interp-st)))
+             (stack)
+             (b* ((stack (stack-push-frame stack)))
+               (stack-set-bindings bindings stack))
+             interp-st))
+
+(define interp-st-push-minor-frame (interp-st)
+  :enabled t
+  :inline t
+  (stobj-let ((stack (interp-st->stack interp-st)))
+             (stack)
+             (b* ((bindings (stack-minor-bindings stack))
+                  (stack (stack-push-minor-frame stack)))
+               (stack-set-minor-bindings bindings stack))
+             interp-st))
+
+(define interp-st-set-debug (debug interp-st)
+  :enabled t
+  :inline t
+  (stobj-let ((stack (interp-st->stack interp-st)))
+             (stack)
+             (stack-set-debug debug stack)
+             interp-st))
+
+(define interp-st-set-minor-debug (debug interp-st)
+  :enabled t
+  :inline t
+  (stobj-let ((stack (interp-st->stack interp-st)))
+             (stack)
+             (stack-set-minor-debug debug stack)
+             interp-st))
+
+
+(define interp-st-decrement-reclimit (interp-st)
+  :guard (posp (interp-st->reclimit interp-st))
+  (update-interp-st->reclimit (1- (interp-st->reclimit interp-st)) interp-st))
+
+(define interp-st-increment-reclimit (interp-st)
+  (update-interp-st->reclimit (1+ (lnfix (interp-st->reclimit interp-st))) interp-st))
+
+
+
+
+;; Interp-st-bind:
+;;
+;; This works differently from a regular LET* or something.  Instead of
+;; containing an expression whose value is returned, this splices some bindings
+;; in between bindings that set some interp-st slots to new values and restore
+;; them to their old values.  E.g.:
+;;   (b* (...
+;;        ((interp-st-bind
+;;          (flags new-flag-expr flag-backup-var)
+;;          (equiv-contexts new-equiv-contexts-expr))
+;;         ((gl-interp-recursive-call err successp-interp-st state)
+;;          (gl-rewrite-relieve-hyps rule.hyps interp-st state)))
+;;        ...)
+;;     ...)
+;; Note: The bindings are of the form
+;;        (slot-name new-value-expr &optional backup-varname)
+;; If backup-varname is specified, it should be already bound to the current value of that slot.
+;; Slot is accessed with interp-st->[slotname] and updated with update-interp-st->[slotname].
+
+
+
+(define interp-st-bind-default-backup-name (slotname)
+  :mode :program
+  (intern-in-package-of-symbol
+   (concatenate 'string "CURRENT-INTERP-ST-" (symbol-name slotname))
+   'fgl::gl-package-symbol))
+
+(define interp-st-accessor (slotname)
+  :mode :program
+  (acl2::tmpl-sym-sublis `(("<FIELD>" . ,(symbol-name slotname)))
+                         'interp-st-><field>
+                         'fgl::gl-package))
+
+(define interp-st-updater (slotname)
+  :mode :program
+  (acl2::tmpl-sym-sublis `(("<FIELD>" . ,(symbol-name slotname)))
+                         'update-interp-st-><field>
+                         'fgl::gl-package))
+
+(define interp-st-bind-backup-vals (args interp-st-name)
+  :mode :program
+  (b* (((when (atom args)) nil)
+       (arg (car args))
+       ((when (eql (len arg) 3))
+        (interp-st-bind-backup-vals (cdr args) interp-st-name))
+       ((list slotname ?expr) arg)
+       (backup-name (interp-st-bind-default-backup-name slotname)))
+    (cons `(,backup-name (,(interp-st-accessor slotname) ,interp-st-name))
+          (interp-st-bind-backup-vals (cdr args) interp-st-name))))
+
+(define interp-st-bind-new-vals (args interp-st-name)
+  :mode :program
+  (b* (((when (atom args)) nil)
+       (arg (car args))
+       ((list slotname expr) arg))
+    (cons `(,interp-st-name (,(interp-st-updater slotname) ,expr ,interp-st-name))
+          (interp-st-bind-new-vals (cdr args) interp-st-name))))
+
+(define interp-st-unbind-vals (args interp-st-name)
+  :mode :program
+  (b* (((when (atom args)) nil)
+       (arg (car args))
+       ((list slotname ?expr backup-name) arg)
+       (backup-name (or backup-name (interp-st-bind-default-backup-name slotname))))
+    (cons `(,interp-st-name (,(interp-st-updater slotname) ,backup-name ,interp-st-name))
+          (interp-st-unbind-vals (cdr args) interp-st-name))))
+
+(def-b*-binder interp-st-bind
+  :body
+  `(b* (,@(interp-st-bind-backup-vals args 'interp-st)
+        ,@(interp-st-bind-new-vals args 'interp-st)
+        ,@forms
+        ,@(interp-st-unbind-vals args 'interp-st))
+     ,rest-expr))
+
+
+
+(define interp-st-bfr-p (x &key (interp-st 'interp-st))
+  :enabled t
+  (stobj-let ((logicman (interp-st->logicman interp-st)))
+             (ok)
+             (lbfr-p x)
+             ok))
+
+(define interp-st-bfr-not (x &key (interp-st 'interp-st))
+  :enabled t
+  :inline t
+  :guard (interp-st-bfr-p x)
+  (stobj-let ((logicman (interp-st->logicman interp-st)))
+             (not)
+             (bfr-not x)
+             not))
