books/centaur/fgl/interp.lisp
@@ -35,7 +35,7 @@
 (include-book "bfr-arithmetic")
 (include-book "glcp-unify-defs")
 (include-book "centaur/meta/bindinglist" :dir :system)
-
+(include-book "syntax-bind")
 ;; (define glcp-unify-alist-bfrlist ((x glcp-unify-alist-p))
 ;;   :measure (len (glcp-unify-alist-fix x))
 ;;   (b* ((x (glcp-unify-alist-fix x))
@@ -91,117 +91,6 @@
     :otherwise nil))
 
 
-(define interp-st-bindings (interp-st)
-  :enabled t
-  :inline t
-  (stobj-let ((stack (interp-st->stack interp-st)))
-             (bindings)
-             (stack-bindings stack)
-             bindings))
-
-(define interp-st-stack-len (interp-st)
-  :enabled t
-  :inline t
-  (stobj-let ((stack (interp-st->stack interp-st)))
-             (len)
-             (stack-len stack)
-             len))
-
-(define interp-st-pop-frame (interp-st)
-  :enabled t
-  :inline t
-  :guard (< 1 (interp-st-stack-len interp-st))
-  (stobj-let ((stack (interp-st->stack interp-st)))
-             (stack)
-             (stack-pop-frame stack)
-             interp-st))
-
-(define interp-st-push-scratch ((x gl-object-p)
-                                interp-st)
-  :enabled t
-  :inline t
-  :guard (< 1 (interp-st-stack-len interp-st))
-  (stobj-let ((stack (interp-st->stack interp-st)))
-             (stack)
-             (stack-push-scratch x stack)
-             interp-st))
-
-(define interp-st-scratch-len (interp-st)
-  :enabled t
-  :inline t
-  (stobj-let ((stack (interp-st->stack interp-st)))
-             (len)
-             (stack-scratchlen stack)
-             len))
-
-(define interp-st-pop-scratch ((n natp)
-                                interp-st)
-  :enabled t
-  :inline t
-  :guard (<= n (interp-st-scratch-len interp-st))
-  (stobj-let ((stack (interp-st->stack interp-st)))
-             (stack)
-             (stack-pop-scratch n stack)
-             interp-st))
-
-(define interp-st-peek-scratch ((n natp)
-                                interp-st)
-  :enabled t
-  :inline t
-  :guard (<= n (interp-st-scratch-len interp-st))
-  (stobj-let ((stack (interp-st->stack interp-st)))
-             (args)
-             (stack-peek-scratch n stack)
-             args))
-
-(define interp-st-add-bindings ((x gl-object-alist-p)
-                                interp-st)
-  :enabled t
-  :inline t
-  (stobj-let ((stack (interp-st->stack interp-st)))
-             (stack)
-             (stack-add-bindings x stack)
-             interp-st))
-
-(define interp-st-set-bindings ((x gl-object-alist-p)
-                                interp-st)
-  :enabled t
-  :inline t
-  (stobj-let ((stack (interp-st->stack interp-st)))
-             (stack)
-             (stack-set-bindings x stack)
-             interp-st))
-
-(define interp-st-push-frame ((bindings gl-object-alist-p)
-                              interp-st)
-  :enabled t
-  :inline t
-  (stobj-let ((stack (interp-st->stack interp-st)))
-             (stack)
-             (b* ((stack (stack-push-frame stack)))
-               (stack-set-bindings bindings stack))
-             interp-st))
-
-(define interp-st-dup-frame (interp-st)
-  :enabled t
-  :inline t
-  (stobj-let ((stack (interp-st->stack interp-st)))
-             (stack)
-             (b* ((bindings (stack-bindings stack))
-                  (stack (stack-push-frame stack)))
-               (stack-set-bindings bindings stack))
-             interp-st))
-
-
-
-
-(define interp-st-decrement-reclimit (interp-st)
-  :guard (posp (interp-st->reclimit interp-st))
-  (update-interp-st->reclimit (1- (interp-st->reclimit interp-st)) interp-st))
-
-(define interp-st-increment-reclimit (interp-st)
-  (update-interp-st->reclimit (1+ (lnfix (interp-st->reclimit interp-st))) interp-st))
-
 (fty::defbitstruct gl-function-mode
   ((dont-concrete-exec booleanp)
    (dont-expand-def booleanp)
@@ -254,6 +143,79 @@
      ,rest-expr))
 
 
+(define gl-interp-time$-arg ((arg gl-object-p) (x pseudo-termp))
+  (b* ((arg (gl-object-case arg :g-concrete (and (true-listp arg.val) arg.val) :otherwise nil))
+       (term-descrip (pseudo-term-case x :fncall x.fn :otherwise x)))
+    (if arg
+        (b* ((msg (nth 3 arg)))
+          (if msg
+              arg
+            (append (take 3 arg)
+                    (list "Gl-interp ~x0: ~st real, ~sc cpu, ~sa bytes~%"
+                          (list term-descrip)))))
+      (list 0 nil nil "Gl-interp ~x0: ~st real, ~sc cpu, ~sa bytes~%"
+            (list term-descrip)))))
+
+(local (defthm assoc-when-key
+         (implies k
+                  (equal (assoc k a)
+                         (hons-assoc-equal k a)))))
+
+(define match-syntax-bind-synp ((synp pseudo-termp))
+  :returns (mv ok (form pseudo-termp) untrans)
+  (b* (((mv ok alist) (cmr::pseudo-term-unify '(synp nil untrans-form trans-form)
+                                              synp nil))
+       ((unless ok) (mv nil nil nil))
+       (untrans-form (cdr (assoc 'untrans-form alist)))
+       (trans-form   (cdr (assoc 'trans-form alist)))
+       ((unless (and (pseudo-term-case untrans-form :quote)
+                     (pseudo-term-case trans-form :quote)))
+        (mv nil nil nil))
+       (val (acl2::pseudo-term-quote->val trans-form)))
+    (if (pseudo-termp val)
+        (mv t val untrans-form)
+      (mv nil nil nil))))
+
+
+         
+
+(define gl-interp-syntax-bind ((synp-arg pseudo-termp)
+                               (x pseudo-termp)
+                               interp-st
+                               state)
+  :returns (mv err
+               (ans gl-object-p)
+               new-interp-st
+               new-state)
+  :prepwork ((local (defthm symbol-alistp-when-gl-object-alist-p
+                      (implies (gl-object-alist-p x)
+                               (symbol-alistp x))
+                      :hints(("Goal" :in-theory (enable gl-object-alist-p))))))
+  (b* (((mv synp-ok synp-term untrans) (match-syntax-bind-synp synp-arg))
+       ((unless (and synp-ok (pseudo-term-case x :var)))
+        ;; We could go ahead and simulate x anyway but this does seem like an error.
+        (mv (gl-msg "Bad syntax-bind form: args ~x0, ~x1." synp-arg x)
+            nil interp-st state))
+       (varname (acl2::pseudo-term-var->name x))
+       (bindings (append (interp-st-minor-bindings interp-st)
+                         (interp-st-bindings interp-st)))
+       ((when (assoc-eq varname bindings))
+        (mv (gl-msg "Syntax-bind error: ~x0 was supposed to be bound in a ~
+                       syntax-bind form but was already bound" varname)
+            nil interp-st state))
+       ((mv ok val) (acl2::magic-ev synp-term bindings state t t))
+       ((unless ok)
+        (mv (gl-msg "Syntax-bind error: ~x0 failed to evaluate -- translated: ~x1" untrans synp-term)
+            nil interp-st state))
+       (val-obj (g-concrete val))
+       (interp-st (interp-st-add-binding varname val-obj interp-st)))
+    (mv nil val-obj interp-st state)))
+
+
+(define gl-interp-or-test-equiv-contexts ((contexts equiv-contextsp))
+  :returns (new-contexts equiv-contextsp)
+  (and (equal contexts '(iff)) '(iff)))
+
 (defines gl-interp
   (define gl-interp-test ((x pseudo-termp)
                           interp-st
@@ -267,14 +229,13 @@
                  (xobj gl-object-p)
                  new-interp-st
                  new-state)
-    (b* ((current-equiv-contexts (interp-st->equiv-contexts interp-st))
-         (interp-st (interp-st-update-equiv-contexts '(iff) interp-st))
-         ((gl-interp-recursive-call err xobj interp-st state)
-          (gl-interp-term-equivs x interp-st state))
-         (interp-st (interp-st-update-equiv-contexts current-equiv-contexts interp-st))
+    (b* (((interp-st-bind
+           (equiv-contexts '(iff)))
+          ((gl-interp-recursive-call err xobj interp-st state)
+           (gl-interp-term-equivs x interp-st state)))
          ((when err)
           (mv err nil interp-st state)))
-      (simplify-if-test xobj interp-st state)))
+      (gl-interp-simplify-if-test xobj interp-st state)))
 
   (define gl-interp-term-equivs ((x pseudo-termp)
                                  interp-st
@@ -311,37 +272,44 @@
     (b* ((interp-st (interp-st-fix interp-st)))
       (pseudo-term-case x
         :const (glcp-value (g-concrete x.val))
-        :var (b* ((bindings (interp-st->bindings interp-st)))
-               (glcp-value (cdr (hons-assoc-equal x.name bindings))))
+        :var (b* ((minor-look (assoc-eq x.name (interp-st-minor-bindings interp-st)))
+                  ((when minor-look)
+                   (glcp-value (cdr minor-look))))
+               (glcp-value (cdr (assoc-eq x.name (interp-st-bindings interp-st)))))
         :lambda
         (b* (((mv x-bindings body) (lambda-nest-to-bindinglist x))
-             (interp-st (interp-st-dup-frame interp-st))
-             (contexts (interp-st->equiv-contexts interp-st))
-             (interp-st (update-interp-st->contexts nil interp-st))
-             ((gl-interp-recursive-call err interp-st state)
-              ;; replaces the top of stack with the bindings
-              (gl-interp-bindinglist bindings interp-st state))
-             (interp-st (upate-interp-st->equiv-contexts contexts interp-st))
+             (interp-st (interp-st-push-minor-frame interp-st))
+             (interp-st (interp-st-set-minor-debug x interp-st))
+             ((interp-st-bind
+               (equiv-contexts nil))
+              ((gl-interp-recursive-call err interp-st state)
+               ;; replaces the top of stack with the bindings
+               (gl-interp-bindinglist bindings interp-st state)))
+
              ((when err)
-              (b* ((interp-st (interp-st-pop-frame interp-st)))
+              (b* ((interp-st (interp-st-pop-minor-frame interp-st)))
                 (mv err nil interp-st state)))
              ((mv err val interp-st state)
               (gl-interp-term-equivs body interp-st state))
-             (interp-st (interp-st-pop-frame interp-st)))
+             (interp-st (interp-st-pop-minor-frame interp-st)))
           (mv err val interp-st state))
         :fncall 
         (b* (((when (and** (eq x.fn 'if) (eql (len x.args) 3)))
-              (gl-interp-if (first x.args)
-                            (second x.args)
-                            (third x.args)
-                            interp-st state))
+              (gl-interp-if/or (first x.args)
+                               (second x.args)
+                               (third x.args)
+                               interp-st state))
              ((when (and** (eq x.fn 'return-last) (eql (len x.args) 3)))
               (gl-interp-return-last (first x.args)
                                      (second x.args)
                                      (third x.args)
                                      interp-st state))
-             ((gl-interp-recursive-call err interp-st state)
-              (gl-interp-arglist x.args interp-st state))
+             ((interp-st-bind
+               (equiv-contexts nil))
+              ((gl-interp-recursive-call err interp-st state)
+               ;; pushes the results from the args onto the scratch frame
+               (gl-interp-arglist x.args interp-st state)))
+
              ((when err)
               (mv err nil interp-st state)))
           (gl-interp-fncall x.fn (len x.args) interp-st state)))))
@@ -379,7 +347,7 @@
          (argslen (len x1.args))
          (args (interp-st-peek-scratch argslen interp-st))
          (interp-st (interp-st-pop-scratch argslen interp-st))
-         (interp-st (interp-st-add-bindings (pairlis$ x1.formals args) interp-st)))
+         (interp-st (interp-st-add-minor-bindings (pairlis$ x1.formals args) interp-st)))
       (gl-interp-bindinglist (cdr bindings) interp-st state)))
          
   (define gl-interp-fncall ((fn pseudo-fnsym-p)
@@ -388,6 +356,10 @@
                             state)
     :measure (list (nfix (interp-st->reclimit interp-st))
                    0 0 1)
+    :returns (mv err
+                 (ans gl-object-p)
+                 new-interp-st
+                 new-state)
     (b* (((gl-function-mode fn-mode)
           (gl-function-mode-fix!
            (cdr (hons-assoc-equal fn (table-alist 'gl-fn-modes (w state))))))
@@ -397,8 +369,13 @@
           (fncall-try-concrete-eval fn args fn-mode.dont-concrete-exec state))
          ((when successp)
           (mv nil ans interp-st state))
-         ((gl-interp-recursive-call err successp ans interp-st state)
-          (gl-rewrite-fncall fn args fn-mode.dont-rewrite interp-st state))
+         (reclimit (interp-st->reclimit interp-st))
+         ((when (zp reclimit))
+          (mv (gl-msg "The recursion limit ran out.") nil interp-st state))
+         ((interp-st-bind
+           (reclimit (1- reclimit) reclimit))
+          ((gl-interp-recursive-call err successp ans interp-st state)
+           (gl-rewrite-fncall fn args fn-mode.dont-rewrite interp-st state)))
          ((when err)
           (mv err nil interp-st state))
          ((when successp)
@@ -407,8 +384,10 @@
           (gl-primitive-fncall fn args fn-mode.dont-primitive-exec interp-st state))
          ((when successp)
           (mv nil ans interp-st state))
-         ((mv err successp ans interp-st state)
-          (gl-interp-fn-definition fn args fn-mode.dont-expand-def interp-st state))
+         ((interp-st-bind
+           (reclimit (1- reclimit) reclimit))
+          ((mv err successp ans interp-st state)
+           (gl-interp-fn-definition fn args fn-mode.dont-expand-def interp-st state)))
          ((when err)
           (mv err nil interp-st state))
          ((when successp)
@@ -420,7 +399,7 @@
                                    (dont)
                                    interp-st
                                    state)
-    :measure (list (nfix (interp-st->reclimit interp-st)) 0 0 0)
+    :measure (list (nfix (interp-st->reclimit interp-st)) 20000 0 0)
     :returns (mv err successp
                  (ans gl-object-p)
                  new-interp-st
@@ -435,16 +414,11 @@
           (mv (gl-msg "Error interpreting a call of ~x0: it was given ~x1 arguments but has ~x2 formals."
                    fn arity (len formals))
               nil nil interp-st state))
-         ((when (zp (interp-st->reclimit interp-st)))
-          (mv (gl-msg "The recursion limit ran out.")
-              nil nil interp-st state))
-         (interp-st (interp-st-push-frame interp-st))
-         (interp-st (interp-st-set-bindings (pairlis$ formals args) interp-st))
-         (interp-st (interp-st-decrement-reclimit interp-st))
+         (interp-st (interp-st-push-frame (pairlis$ formals args) interp-st))
+         (interp-st (interp-st-set-debug fn interp-st))
          ((mv err ans interp-st state)
           (gl-interp-term-equivs body interp-st state))
-         (interp-st (interp-st-pop-frame interp-st))
-         (interp-st (interp-st-increment-reclimit interp-st)))
+         (interp-st (interp-st-pop-frame interp-st)))
       (mv err ans interp-st state)))
 
 
@@ -453,36 +427,303 @@
                              (dont)
                              interp-st
                              state)
-    :measure (list (nfix (interp-st->reclimit interp-st)) 0 0 0)
+    :measure (list (nfix (interp-st->reclimit interp-st)) 20000 0 0)
     :returns (mv err successp
                  (ans gl-object-p)
                  new-interp-st
                  new-state)
     (b* (((when dont)
           (mv nil nil nil interp-st state))
-         (backchain-limit (interp-st->backchain-limit interp-st))
-         ((when (eql 0 backchain-limit))
-          (mv nil nil nil interp-st state))
-         (interp-st (update-interp-st->backchain-limit (1- backchain-limit) interp-st))
          (rules (fn-rewrite-rules fn (glcp-config->rewrite-rule-table
                                       (interp-st->config interp-st))
                                   (w state)))
-         ;; Pushes a stack frame if successful!
-         ((gl-interp-recursive-call err successp rhs interp-st state)
-          (gl-rewrite-fncall-rules rules fn args interp-st state))
+         ((unless rules)
+          (mv nil nil nil interp-st state))
+         (reclimit (interp-st->reclimit interp-st))
+         ((when (zp reclimit))
+          (mv (gl-msg "The recursion limit ran out.")
+              nil nil interp-st state)))
+      (gl-rewrite-try-rules rules fn args interp-st state)))
 
+  (define gl-rewrite-try-rules ((rules pseudo-rewrite-rule-listp)
+                                (fn pseudo-fnsym-p)
+                                (args gl-objectlist-p)
+                                interp-st
+                                state)
+    :measure (list (nfix (interp-st->reclimit interp-st)) 10000 (len rules) 0)
+    :returns (mv err successp
+                 (ans gl-object-p)
+                 new-interp-st
+                 new-state)
+    (b* (((when (atom rules))
+          (mv nil nil nil interp-st state))
+         ((gl-interp-recursive-call err successp ans interp-st state)
+          (gl-rewrite-try-rule (car rules) fn args interp-st state))
+         ((when (or err successp))
+          (mv err successp ans interp-st state)))
+      (gl-rewrite-try-rules (cdr rules) fn args interp-st state)))
 
+  (define gl-rewrite-try-rule ((rule pseudo-rewrite-rule-p)
+                               (fn pseudo-fnsym-p)
+                               (args gl-objectlist-p)
+                               interp-st
+                               state)
+    :measure (list (nfix (interp-st->reclimit interp-st)) 10000 0 0)
+    :returns (mv err successp
+                 (ans gl-object-p)
+                 new-interp-st
+                 new-state)
+    (b* (((acl2::rewrite-rule rule))
+         ((unless (and** (mbt (and* (symbolp rule.equiv)
+                                    (not (eq rule.equiv 'quote))
+                                    ;; (ensure-equiv-relationp rule.equiv (w state))
+                                    (not (eq rule.subclass 'acl2::meta))
+                                    (pseudo-termp rule.lhs)))
+                         (pseudo-term-case rule.lhs :fncall (eq rule.lhs.fn (pseudo-fnsym-fix fn)))))
+          (mv (gl-msg "Malformed rewrite rule: ~x0~%" rule)
+              nil nil interp-st state))
+         ((unless (or (eq rule.equiv 'equal)
+                      ;; bozo check refinements
+                      (member rule.equiv (interp-st->equiv-contexts interp-st))))
+          (mv nil nil nil interp-st state))
+         (rule.lhs.args (pseudo-term-call->args rule.lhs))
+         ((mv unify-ok bindings) (glcp-unify-term/gobj-list rule.lhs.args args nil))
+         ((unless unify-ok) (mv nil nil nil interp-st state))
+         ((unless (mbt (pseudo-term-listp rule.hyps)))
+          (mv (gl-msg "Malformed rewrite rule: ~x0~%" rule)
+              nil nil interp-st state))
+         (backchain-limit (interp-st->backchain-limit interp-st))
+         ((when (and* rule.hyps (eql 0 backchain-limit)))
+          (mv nil nil nil interp-st state))
+         (flags (interp-st->flags interp-st))
+         (hyps-flags  (!interp-st->intro-bvars
+                       t
+                       (!interp-flags->intro-bvars
+                        nil
+                        (!interp-flags->simplify-logic nil flags))))
+         (interp-st (interp-st-push-frame bindings interp-st))
+         (interp-st (interp-st-set-debug rule interp-st))
+         ((interp-st-bind
+           (flags hyps-flags flags)
+           (contexts '(iff))
+           (backchain-limit (1- backchain-limit) backchain-limit))
+          ((gl-interp-recursive-call err successp interp-st state)
+           (gl-rewrite-relieve-hyps rule.hyps interp-st state)))
 
+         ((unless successp)
+          (b* ((interp-st (interp-st-pop-frame interp-st)))
+            (mv err nil nil interp-st state)))
+
+         (concl-flags (!interp-st->intro-bvars t flags))
+         ((interp-st-bind
+           (flags concl-flags flags))
+          ((mv err val interp-st state)
+           (gl-interp-term-equivs rule.rhs interp-st state)))
+
+         (interp-st (interp-st-pop-frame interp-st)))
+
+      (mv err (not err) val interp-st state)))
+          
+    
+  (define gl-interp-time$ ((timing-arg pseudo-termp)
+                           (x pseudo-termp)
+                           interp-st
+                           state)
+    :measure (list (nfix (interp-st->reclimit interp-st)) 2020
+                   (+ (pseudo-term-binding-count first-arg)
+                      (pseudo-term-binding-count last-arg))
+                   30)
+    :returns (mv err
+                 (ans gl-object-p)
+                 new-interp-st
+                 new-state)
+    (b* (((interp-st-bind
+           (equiv-contexts nil))
+          ((gl-interp-recursive-call err time$-arg interp-st state)
+           (gl-interp-term-equivs timing-arg interp-st state)))
+         ((when err)
+          (mv err nil interp-st state))
+         (time$-arg (gl-interp-time$-arg time$-arg x)))
+      (time$1 time$-arg
+              (gl-interp-term-equivs x interp-st state))))
          
+  (define gl-interp-return-last ((return-last-fnname pseudo-termp)
+                                 (first-arg pseudo-termp)
+                                 (last-arg pseudo-termp)
+                                 interp-st state)
+    :measure (list (nfix (interp-st->reclimit interp-st)) 2020
+                   (+ (pseudo-term-binding-count first-arg)
+                      (pseudo-term-binding-count last-arg))
+                   40)
+    :returns (mv err
+                 (ans gl-object-p)
+                 new-interp-st
+                 new-state)
+    (b* (((when (equal return-last-fnname ''time$1-raw))
+          (gl-interp-time$ first-arg last-arg interp-st state))
+         ((when (equal return-last-fnname ''(syntax-bind)))
+          (gl-interp-syntax-bind first-arg last-arg interp-st state)))
+      ;; Otherwise just evaluate the last-arg.
+      (gl-interp-term-equivs last-arg interp-st state)))
+                
+               
 
-              ((when (zp (interp-st->reclimit interp-st)))
-          (glcp-interp-error (gl-msg "The recursion limit ran out.")))
-         (interp-st (interp-st-decrement-reclimit interp-st))
-         
-         
-  gl-interp-if
-  gl-interp-return-last
-  gl-rewrite-fncall)
+  (define gl-interp-if/or ((test pseudo-termp)
+                           (then pseudo-termp)
+                           (else pseudo-termp)
+                           interp-st
+                           state)
+    :measure (list (nfix (interp-st->reclimit interp-st))
+                   2020
+                   (+ (pseudo-term-binding-count test)
+                      (pseudo-term-binding-count then)
+                      (pseudo-term-binding-count else))
+                   60)
+    :returns (mv err
+                 (ans gl-object-p)
+                 new-interp-st
+                 new-state)
+    (if (hons-equal test then)
+        (gl-interp-or test else interp-st state)
+      (gl-interp-if test then else interp-st state)))
+
+  
+  (define gl-interp-if ((test pseudo-termp)
+                        (then pseudo-termp)
+                        (else pseudo-termp)
+                        interp-st
+                        state)
+    :measure (list (nfix (interp-st->reclimit interp-st))
+                   2020
+                   (+ (pseudo-term-binding-count test)
+                      (pseudo-term-binding-count then)
+                      (pseudo-term-binding-count else))
+                   40)
+    :returns (mv err
+                 (ans gl-object-p)
+                 new-interp-st
+                 new-state)
+    ;; Tricky because we have to keep the test/thenval on the stack while we
+    ;; run the then/else branches, because we might simplify the logicman while
+    ;; running them.
+    (b* (((gl-interp-recursive-call err testbfr interp-st state)
+          (gl-interp-test test interp-st state))
+         ((when err) (mv err nil interp-st state))
+         (interp-st (interp-st-push-bool-scratch testbfr interp-st))
+         ((gl-interp-recursive-call err then-unreachable thenval interp-st state)
+         ;; pushes val onto scratch if not unreachable
+          (gl-maybe-interp testbfr then interp-st state))
+         ((when err)
+          (b* ((interp-st (interp-st-pop-bool-scratch 1 interp-st)))
+            (mv err nil interp-st state)))
+         (interp-st (interp-st-push-scratch thenval interp-st))
+         ;; note: testbool may have changed if we simplified the logicman
+         (testbfr (first (interp-st-bool-scratch interp-st)))
+         ((gl-interp-recursive-call err else-unreachable elseval interp-st state)
+          ;; pushes val onto scratch if not unreachable
+          (gl-maybe-interp (interp-st-bfr-not testbfr interp-st) else interp-st state))
+         ((when err)
+          (b* ((interp-st (interp-st-pop-scratch 1 interp-st))
+               (interp-st (interp-st-pop-bool-scratch 1 interp-st)))
+            (mv err nil interp-st state)))
+         (thenval (first (interp-st-scratch interp-st)))
+         (testbfr (first (interp-st-bool-scratch interp-st)))
+         (interp-st (interp-st-pop-scratch 1 interp-st))
+         (interp-st (interp-st-pop-bool-scratch 1 interp-st))
+         ((when then-unreachable)
+          (if else-unreachable
+              (mv :unreachable nil interp-st state)
+            (mv nil elseval interp-st state)))
+         ((when else-unreachable)
+          (mv nil thenval interp-st state)))
+      (gl-interp-merge-branches testbfr thenval elseval interp-st state)))
+
+  (define gl-interp-or ((test pseudo-termp)
+                        (else pseudo-termp)
+                        interp-st
+                        state)
+    :measure (list (nfix (interp-st->reclimit interp-st))
+                   2020
+                   (+ (pseudo-term-binding-count test)
+                      (pseudo-term-binding-count else))
+                   40)
+    :returns (mv err
+                 (ans gl-object-p)
+                 new-interp-st
+                 new-state)
+    (b* ((equiv-contexts (interp-st->equiv-contexts interp-st))
+         (or-test-equiv-contexts (gl-interp-or-test-equiv-contexts equiv-contexts))
+         ((interp-st-let
+           (equiv-contexts or-test-equiv-contexts equiv-contexts))
+          ((gl-interp-recursive-call err testval interp-st state)
+           (gl-interp-term-equivs test interp-st state)))
+         ((when err) (mv err nil interp-st state))
+         ((mv err testbfr interp-st state)
+          (gl-interp-simplify-if-test testval interp-st state))
+         ((when err) (mv err nil interp-st state))
+         (interp-st (interp-st-push-scratch testval interp-st))
+         (interp-st (interp-st-push-bool-scratch testbfr interp-st))
+         ((gl-interp-recursive-call err else-unreachable elseval interp-st state)
+          ;; pushes val onto scratch if not unreachable
+          (gl-maybe-interp (interp-st-bfr-not testbfr interp-st) else interp-st state))
+         (testval (first (interp-st-scratch interp-st)))
+         (testbfr (first (interp-st-bool-scratch interp-st)))
+         (interp-st (interp-st-pop-scratch 1 interp-st))
+         (interp-st (interp-st-pop-bool-scratch 1 interp-st))
+         ((when err)
+          (mv err nil interp-st state))
+         ((when else-unreachable)
+          (mv nil testval interp-st state)))
+      (gl-interp-merge-branches testbfr testval elseval interp-st state)))
+
+
+  (define gl-maybe-interp ((test interp-st-bfr-p)
+                           (x pseudo-termp)
+                           interp-st
+                           state)
+    :measure (list (nfix (interp-st->reclimit interp-st))
+                   2020
+                   (pseudo-term-binding-count x)
+                   40)
+    :returns (mv err
+                 unreachable
+                 (ans gl-object-p)
+                 new-interp-st
+                 new-state)
+    (b* (((mv contra checkpoint interp-st)
+          (stobj-let ((logicman (interp-st->logicman interp-st))
+                      (pathcond (interp-st->pathcond interp-st))
+                      (constraint-pathcond (interp-st->constraint interp-st)))
+                     (contra checkpoint pathcond constraint-pathcond)
+                     ;; this is a bit weak... would be better to check against
+                     ;; both constraint and pathcond at once somehow
+                     (b* ((bfr-mode  (logicman->mode logicman))
+                          (checkpoint (pathcond-checkpoint bfr-mode pathcond))
+                          ((mv constraint-implies constraint-pathcond)
+                           (logicman-pathcond-implies test constraint-pathcond))
+                          ((when constraint-implies)
+                           (mv (eql constraint-implies 0) checkpoint pathcond constraint-pathcond))
+                          ((mv contra pathcond) (logicman-pathcond-assume test pathcond))
+                          ((when contra)
+                           (b* ((pathcond (pathcond-rewind checkpoint bfr-mode pathcond)))
+                             (mv contra nil pathcond constraint-pathcond))))
+                       (mv nil checkpoint pathcond constraint-pathcond))
+                     (mv contra checkpoint interp-st)))
+         ((when contra)
+          (mv nil t nil interp-st state))
+         ((mv err ans interp-st state)
+          (gl-interp-term-equivs x interp-st state))
+         (interp-st (stobj-let ((logicman (interp-st->logicman interp-st))
+                                (pathcond (interp-st->pathcond interp-st)))
+                               (pathcond)
+                               (pathcond-rewind checkpoint (logicman->bfr-mode logicman) pathcond)
+                               interp-st))
+         ((when (eq err :unreachable))
+          (mv nil t nil interp-st state)))
+      (mv err nil ans interp-st state)))
+
+    gl-interp-merge-branches
+    gl-interp-simplify-if-test)
              
         
          
