books/centaur/fgl/syntax-bind.lisp
@@ -1,0 +1,90 @@
+; GL - A Symbolic Simulation Framework for ACL2
+; Copyright (C) 2019 Centaur Technology
+;
+; Contact:
+;   Centaur Technology Formal Verification Group
+;   7600-C N. Capital of Texas Highway, Suite 300, Austin, TX 78731, USA.
+;   http://www.centtech.com/
+;
+; License: (An MIT/X11-style license)
+;
+;   Permission is hereby granted, free of charge, to any person obtaining a
+;   copy of this software and associated documentation files (the "Software"),
+;   to deal in the Software without restriction, including without limitation
+;   the rights to use, copy, modify, merge, publish, distribute, sublicense,
+;   and/or sell copies of the Software, and to permit persons to whom the
+;   Software is furnished to do so, subject to the following conditions:
+;
+;   The above copyright notice and this permission notice shall be included in
+;   all copies or substantial portions of the Software.
+;
+;   THE SOFTWARE IS PROVIDED "AS IS", WITHOUT WARRANTY OF ANY KIND, EXPRESS OR
+;   IMPLIED, INCLUDING BUT NOT LIMITED TO THE WARRANTIES OF MERCHANTABILITY,
+;   FITNESS FOR A PARTICULAR PURPOSE AND NONINFRINGEMENT. IN NO EVENT SHALL THE
+;   AUTHORS OR COPYRIGHT HOLDERS BE LIABLE FOR ANY CLAIM, DAMAGES OR OTHER
+;   LIABILITY, WHETHER IN AN ACTION OF CONTRACT, TORT OR OTHERWISE, ARISING
+;   FROM, OUT OF OR IN CONNECTION WITH THE SOFTWARE OR THE USE OR OTHER
+;   DEALINGS IN THE SOFTWARE.
+;
+; Original author: Sol Swords <sswords@centtech.com>
+
+(in-package "FGL")
+
+(include-book "centaur/meta/unify" :dir :system)
+
+;; note: probably need to put this somewhere else
+(defmacro syntax-bind (dummy-var form)
+  `(return-last '(syntax-bind)
+                (synp 'nil ',form ',form)
+                ,dummy-var))
+
+(defevaluator synbind-ev synbind-ev-list ((return-last x y z)) :namedp t)
+
+(local (acl2::def-ev-pseudo-term-fty-support synbind-ev synbind-ev-list))
+
+(local (defthm assoc-when-key
+         (implies k
+                  (equal (assoc k a)
+                         (hons-assoc-equal k a)))))
+
+(define match-syntax-bind ((x pseudo-termp))
+  :returns (mv (dummy-var symbolp
+                          ;; note: not pseudo-var-p because we indicate no match by returning nil
+                          :rule-classes :type-prescription)
+               (form pseudo-termp))
+  (b* (((mv ok alist)
+        (cmr::pseudo-term-unify '(return-last '(syntax-bind)
+                                         (synp 'nil untrans-form trans-form)
+                                         dummy-var)
+                           x nil))
+       ((unless ok) (mv nil nil))
+       (untrans-form (cdr (assoc 'untrans-form alist)))
+       (trans-form (cdr (assoc 'trans-form alist)))
+       (dummy-var (cdr (assoc 'dummy-var alist)))
+       ((unless (And (pseudo-term-case dummy-var :var)
+                     (pseudo-term-case untrans-form :quote)
+                     (pseudo-term-case trans-form
+                       :quote (pseudo-termp trans-form.val)
+                       :otherwise nil)))
+        (mv nil nil)))
+    (mv (acl2::pseudo-term-var->name dummy-var)
+        (acl2::pseudo-term-quote->val trans-form)))
+  ///
+  (std::defretd eval-when-<fn>
+    (implies dummy-var
+             (equal (synbind-ev x a)
+                    (cdr (hons-assoc-equal dummy-var a))))
+    :hints(("Goal" :expand ((:free (pat x alist) (cmr::pseudo-term-unify pat x alist))
+                            (:free (pat x alist) (cmr::pseudo-term-list-unify pat x alist))))))
+
+  (fty::deffixequiv match-syntax-bind)
+
+  (local
+   (make-event
+    (b* (((mv err val state) (acl2::translate '(syntax-bind foo (and x y z)) t t nil 'match-syntax-bind-works
+                                        (w state) state))
+         ((when err) (mv err val state)))
+      (value `(defthm match-syntax-bind-works
+                (b* (((mv dummy-var form) (match-syntax-bind ',val)))
+                  (and (equal dummy-var 'foo)
+                       (equal form '(if x (if y z 'nil) 'nil))))))))))
